A12Kernel.lean
@@ -191,6 +191,7 @@ import A12Kernel.Elaboration.AddressedDateRangeBoundPart
 import A12Kernel.Elaboration.AddressedNumberField
 import A12Kernel.Elaboration.CurrentRepetitionComputation
 import A12Kernel.Elaboration.CurrentRepetitionNumberToString
+import A12Kernel.Elaboration.CurrentRepetitionStringToNumber
 import A12Kernel.Elaboration.AddressedNumberAbs
 import A12Kernel.Elaboration.AddressedNumberRound
 import A12Kernel.Elaboration.AddressedNumberExtremum
